works for big params

w64x4/test/main.c
@@ -1,0 +1,139 @@
+#include <stdio.h>
+#include <stdint.h>
+#include <assert.h>
+#include <string.h>
+
+#define NLIMBS 4
+void print_result(uint64_t* x);
+
+
+extern void __addm(uint64_t* r, uint64_t* p, uint64_t* a, uint64_t* b);
+extern void __mulm(uint64_t* r, uint64_t* p, uint64_t* a, uint64_t* b);
+extern void __expm(uint64_t* r, uint64_t* p, uint64_t* a, uint64_t* b);
+
+
+uint64_t tadd[][4][64] =
+ {
+  {  { 0ull , 0ull , 0ull , 0ull, 0ull , 0ull , 0ull , 0ull, 0ull , 0ull , 0ull , 0ull, 0ull , 0ull , 0ull , 0ull, 0ull , 0ull , 0ull , 0ull, 0ull , 0ull , 0ull , 0ull, 0ull , 0ull , 0ull , 0ull, 0ull , 0ull , 0ull , 0ull, 0ull , 0ull , 0ull , 0ull, 0ull , 0ull , 0ull , 0ull, 0ull , 0ull , 0ull , 0ull, 0ull , 0ull , 0ull , 0ull, 0ull , 0ull , 0ull , 0ull, 0ull , 0ull , 0ull , 0ull, 0ull , 0ull , 0ull , 0ull, 0ull , 0ull , 0ull , 0ull }
+     , { 0ull , 0ull , 0ull , 0ull, 0ull , 0ull , 0ull , 0ull, 0ull , 0ull , 0ull , 0ull, 0ull , 0ull , 0ull , 0ull, 0ull , 0ull , 0ull , 0ull, 0ull , 0ull , 0ull , 0ull, 0ull , 0ull , 0ull , 0ull, 0ull , 0ull , 0ull , 0ull, 0ull , 0ull , 0ull , 0ull, 0ull , 0ull , 0ull , 0ull, 0ull , 0ull , 0ull , 0ull, 0ull , 0ull , 0ull , 0ull, 0ull , 0ull , 0ull , 0ull, 0ull , 0ull , 0ull , 0ull, 0ull , 0ull , 0ull , 0ull, 0ull , 0ull , 0ull , 0ull }
+     , { 0ull , 0ull , 0ull , 0ull, 0ull , 0ull , 0ull , 0ull, 0ull , 0ull , 0ull , 0ull, 0ull , 0ull , 0ull , 0ull, 0ull , 0ull , 0ull , 0ull, 0ull , 0ull , 0ull , 0ull, 0ull , 0ull , 0ull , 0ull, 0ull , 0ull , 0ull , 0ull, 0ull , 0ull , 0ull , 0ull, 0ull , 0ull , 0ull , 0ull, 0ull , 0ull , 0ull , 0ull, 0ull , 0ull , 0ull , 0ull, 0ull , 0ull , 0ull , 0ull, 0ull , 0ull , 0ull , 0ull, 0ull , 0ull , 0ull , 0ull, 0ull , 0ull , 0ull , 0ull }
+     , { 0ull , 0ull , 0ull , 0ull, 0ull , 0ull , 0ull , 0ull, 0ull , 0ull , 0ull , 0ull, 0ull , 0ull , 0ull , 0ull, 0ull , 0ull , 0ull , 0ull, 0ull , 0ull , 0ull , 0ull, 0ull , 0ull , 0ull , 0ull, 0ull , 0ull , 0ull , 0ull, 0ull , 0ull , 0ull , 0ull, 0ull , 0ull , 0ull , 0ull, 0ull , 0ull , 0ull , 0ull, 0ull , 0ull , 0ull , 0ull, 0ull , 0ull , 0ull , 0ull, 0ull , 0ull , 0ull , 0ull, 0ull , 0ull , 0ull , 0ull, 0ull , 0ull , 0ull , 0ull }
+   }
+ };
+
+uint64_t tmul[][4][64] =
+ {
+  {  { 0ull , 0ull , 0ull , 0ull, 0ull , 0ull , 0ull , 0ull, 0ull , 0ull , 0ull , 0ull, 0ull , 0ull , 0ull , 0ull, 0ull , 0ull , 0ull , 0ull, 0ull , 0ull , 0ull , 0ull, 0ull , 0ull , 0ull , 0ull, 0ull , 0ull , 0ull , 0ull, 0ull , 0ull , 0ull , 0ull, 0ull , 0ull , 0ull , 0ull, 0ull , 0ull , 0ull , 0ull, 0ull , 0ull , 0ull , 0ull, 0ull , 0ull , 0ull , 0ull, 0ull , 0ull , 0ull , 0ull, 0ull , 0ull , 0ull , 0ull, 0ull , 0ull , 0ull , 0ull }
+     , { 0ull , 0ull , 0ull , 0ull, 0ull , 0ull , 0ull , 0ull, 0ull , 0ull , 0ull , 0ull, 0ull , 0ull , 0ull , 0ull, 0ull , 0ull , 0ull , 0ull, 0ull , 0ull , 0ull , 0ull, 0ull , 0ull , 0ull , 0ull, 0ull , 0ull , 0ull , 0ull, 0ull , 0ull , 0ull , 0ull, 0ull , 0ull , 0ull , 0ull, 0ull , 0ull , 0ull , 0ull, 0ull , 0ull , 0ull , 0ull, 0ull , 0ull , 0ull , 0ull, 0ull , 0ull , 0ull , 0ull, 0ull , 0ull , 0ull , 0ull, 0ull , 0ull , 0ull , 0ull }
+     , { 0ull , 0ull , 0ull , 0ull, 0ull , 0ull , 0ull , 0ull, 0ull , 0ull , 0ull , 0ull, 0ull , 0ull , 0ull , 0ull, 0ull , 0ull , 0ull , 0ull, 0ull , 0ull , 0ull , 0ull, 0ull , 0ull , 0ull , 0ull, 0ull , 0ull , 0ull , 0ull, 0ull , 0ull , 0ull , 0ull, 0ull , 0ull , 0ull , 0ull, 0ull , 0ull , 0ull , 0ull, 0ull , 0ull , 0ull , 0ull, 0ull , 0ull , 0ull , 0ull, 0ull , 0ull , 0ull , 0ull, 0ull , 0ull , 0ull , 0ull, 0ull , 0ull , 0ull , 0ull }
+     , { 0ull , 0ull , 0ull , 0ull, 0ull , 0ull , 0ull , 0ull, 0ull , 0ull , 0ull , 0ull, 0ull , 0ull , 0ull , 0ull, 0ull , 0ull , 0ull , 0ull, 0ull , 0ull , 0ull , 0ull, 0ull , 0ull , 0ull , 0ull, 0ull , 0ull , 0ull , 0ull, 0ull , 0ull , 0ull , 0ull, 0ull , 0ull , 0ull , 0ull, 0ull , 0ull , 0ull , 0ull, 0ull , 0ull , 0ull , 0ull, 0ull , 0ull , 0ull , 0ull, 0ull , 0ull , 0ull , 0ull, 0ull , 0ull , 0ull , 0ull, 0ull , 0ull , 0ull , 0ull }
+   }
+ };
+
+
+
+/* uint64_t tmul[][4][4] = */
+/*  { */
+/*    {  { 7ull , 0ull , 0ull , 0ull } */
+/*     , { 0ull , 0ull , 0ull , 0ull } */
+/*     , { 0ull , 0ull , 0ull , 0ull } */
+/*     , { 0ull , 0ull , 0ull , 0ull } */
+/*    } */
+/*  , {  { 13ull , 13ull , 13ull , 13ull } */
+/*     , { 1ull , 1ull , 1ull , 1ull } */
+/*     , { 1ull , 1ull , 1ull , 1ull } */
+/*     , { 1ull , 1ull , 1ull , 1ull } */
+/*    } */
+/*  , {  { 5ull , 0ull , 0ull , 0ull } */
+/*     , { 3ull , 0ull , 0ull , 0ull } */
+/*     , { 3ull , 0ull , 0ull , 0ull } */
+/*     , { 4ull , 0ull , 0ull , 0ull } */
+/*    } */
+/*  , {  { 100ull , 0ull , 0ull , 0ull } */
+/*     , { 50ull , 0ull , 0ull , 0ull } */
+/*     , { 20ull , 0ull , 0ull , 0ull } */
+/*     , { 0ull , 0ull , 0ull , 0ull } */
+/*    } */
+/*  }; */
+
+
+
+/* uint64_t texp[][3][4] = */
+/*  { */
+/*   {  { 2ull , 3ull , 0ull , 0ull }     // represents: (2*(2^64)^0 + 3 * (2^64)^1 )   */
+/*      , { 2ull , 0ull , 0ull , 0ull }   // represnets: 2 */
+/*      , { 4ull , 12ull , 9ull , 0ull }  // represents: (4*(2^64)^0 + 12 * (2^64)^1 + 9 * (2^64)^2) %% (2^255 - 19) */
+/*    } */
+/*  , {  { 2ull , 3ull , 4ull , 5ull } */
+/*     , { 0ull , 0ull , 0ull , 0ull } */
+/*     , { 1ull , 0ull , 0ull , 0ull } */
+/*    } */
+/*  , {  { 9ull , 9ull , 9ull , 9ull } */
+/*     , { 1ull , 0ull , 0ull , 0ull } */
+/*     , { 9ull , 9ull , 9ull , 9ull } */
+/*    } */
+/*   , {  { 123123ull , 0ull , 0ull , 0ull }  */
+/*     , { 500ull , 0ull , 0ull , 0ull } */
+/*     , { 11117009174922751360ull , 13416253971750811784ull , 7609481284495345029ull , 5760204542479289991ull } */
+/*        /\*  (123123^500) %% (2^255 - 19) = 11117009174922751360 * (2^64)^ 0  */
+/* 	   + 13416253971750811784 * (2^64)^1   */
+/* 	   + 7609481284495345029 * (2^64)^2  */
+/* 	   + 5760204542479289991 * (2^64)^3 *\/ */
+/*    } */
+/*  }; */
+
+
+
+
+int main() {
+  uint64_t result[64]; 
+  int i, b,a;
+
+  printf("Testing ADDM: ");
+  b = 1;
+  for (i=0; i<sizeof(tadd)/sizeof(tadd[0]); i++) {
+    __addm(result, tadd[i][0], tadd[i][1], tadd[i][2]);
+   a = memcmp(result, tadd[i][3], sizeof(tadd[i][3]));
+   b =   b && !a;
+  }
+  if (b) printf("OK\n"); else printf("FAIL!\n");
+
+
+    /* __mulm(result, tmul[3][0], tmul[3][1],tmul[3][2]); */
+    /* print_result(result); */
+  
+  printf("Testing MULM: ");
+  b = 1;
+  for (i=0; i<sizeof(tmul)/sizeof(tmul[0]); i++) {
+    __mulm(result, tmul[i][0], tmul[i][1],tmul[i][2]);
+   a = memcmp(result, tmul[i][3], sizeof(tmul[i][3]));
+   b =   b && !a;
+  }
+  if (b) printf("OK\n"); else printf("FAIL!\n");
+
+
+  /* printf("Testing EXPM: "); */
+  /* b = 1; */
+  /* for (i=0; i<sizeof(tmul)/sizeof(tmul[0]); i++) { */
+  /*   __expm(result, tmul[i][0], tmul[i][1],tmul[i][2]); */
+  /*  a = memcmp(result, tmul[i][3], sizeof(tmul[i][3])); */
+  /*  b =   b && !a; */
+  /* } */
+  /* if (b) printf("OK\n"); else printf("FAIL!\n"); */
+
+  
+  
+  
+  return 0;
+}
+
+
+
+
+void print_result(uint64_t* x) {
+  printf("echo: ");
+  for(int i = 0; i < NLIMBS; i++){
+    printf("%lu ", *(x+(i*sizeof(uint64_t)/sizeof(uint64_t))));
+  }
+  printf("\n");  
+}
