w64x4/proof/Fp_w64x4_proof_mulm.ec
@@ -2,11 +2,11 @@ require import AllCore IntDiv CoreMap List.
 
 require import JModel JBigNum.
 require import Fp_w64x4_spec Fp_w64x4_extract Ith_Bit64.
-import Array28 Array14 Array7.
+import Array128 Array64 Array32.
 import Zp W64x4 R.
 import StdBigop Bigint BIA.
 
-op R : W64.t Array14.t = R2.bn_ofint Ri.
+op R : W64.t Array64.t = R2.bn_ofint Ri.
 require import BarrettRedInt.
 
 lemma kok (a b c : real) : 0%r <= a => 0%r < b => 1%r < c =>
@@ -37,7 +37,7 @@ have q2: Ri < W64x8.modulusR .
   have ->: x = Ri. rewrite /x /Ri /ri. smt().
    smt(@RealExp). smt(@RealExp). smt(P_pos). rewrite exp_lemma1. smt(). smt(). apply q.
     have ->: 2%r ^ (64 * dnlimbs)%r = (2 ^ (64 * dnlimbs))%r. 
-    rewrite - exp_lemma1. smt(). smt(). trivial.
+    rewrite - exp_lemma1. smt(). smt(). smt().
 smt(@Real).
 have ->: (W64x8.valR ((R2.bn_ofint Ri))%R2)%W64x8   = Ri.
 rewrite W64x8.R.bn_ofintK. 
@@ -56,8 +56,8 @@ proc; simplify.
 wp.
 while ( #pre /\ ={r,i} /\ (a,of_0,cf,_zero){1}=(ak,_of,_cf,W64.zero){2} /\ 
         1 <= i{2} <= nlimbs /\ !_of{2}).
- wp; skip => />; smt(Array14.get_setE Array14.set_set_if).
-wp; skip => />; smt (Array14.set_set_if).
+ wp; skip => />; smt(Array64.get_setE Array64.set_set_if).
+wp; skip => />; smt (Array64.set_set_if).
 qed.
 
 
@@ -71,8 +71,8 @@ proof.
 proc. simplify.
 wp. while ( #pre /\ ={i} /\ (aux,_zero){1}=(nlimbs-1,W64.zero){2} /\ 
             0 <= i{2} <= nlimbs-1 /\ kk{1} = k{2}).
- wp; skip => />; smt(Array14.get_setE Array14.set_set_if).
-wp; skip; smt(Array14.get_setE Array14.set_set_if).
+ wp; skip => />; smt(Array64.get_setE Array64.set_set_if).
+wp; skip; smt(Array64.get_setE Array64.set_set_if).
 qed.
 
 
@@ -86,8 +86,8 @@ proc; simplify.
 wp.
 while ( #pre /\ ={r,i} /\ (a,of_0,cf,_zero){1}=(ak,_of,_cf,W64.zero){2} /\ 
         1 <= i{2} <= dnlimbs /\ !_of{2}).
- wp; skip => />; smt(Array28.get_setE Array28.set_set_if).
-wp; skip => />; smt (Array28.set_set_if).
+ wp; skip => />; smt(Array128.get_setE Array128.set_set_if).
+wp; skip => />; smt (Array128.set_set_if).
 qed.
 
 
@@ -101,8 +101,8 @@ proof.
 proc. simplify.
 wp. while ( #pre /\ ={i} /\ (aux,_zero){1}=(dnlimbs-1,W64.zero){2} /\ 
             0 <= i{2} <= dnlimbs-1 /\ kk{1} = k{2}).
- wp; skip => />; smt(Array28.get_setE Array28.set_set_if).
-wp; skip; smt(Array28.get_setE Array28.set_set_if).
+ wp; skip => />; smt(Array128.get_setE Array128.set_set_if).
+wp; skip; smt(Array128.get_setE Array128.set_set_if).
 qed.
 
 
@@ -189,8 +189,8 @@ transitivity
   exlim a{1}, b{1} => aa bb.
   while (={i,b} /\ 1 <= i{2} <= dnlimbs /\ 
          (cf, aa){1}=(c, a){2} /\
-         (forall k, 0 <= k < i{2} => a{1}.[k] = r{2}.[k])%Array14 /\
-         (forall k, i{2} <= k < dnlimbs => a{1}.[k] = aa.[k])%Array14).
+         (forall k, 0 <= k < i{2} => a{1}.[k] = r{2}.[k])%Array64 /\
+         (forall k, i{2} <= k < dnlimbs => a{1}.[k] = aa.[k])%Array64).
    wp; skip => /> &1 &2 Hi1 _ Hh1 Hh2 Hi2.
    split => *; first smt().
    split => *; first smt().
@@ -209,7 +209,7 @@ transitivity
    split => k *.
     by rewrite (_:k=0) 1:/# !set_eqiE /#.
    by rewrite set_neqiE /#.
-  by apply Array14.ext_eq; smt().
+  by apply Array64.ext_eq; smt().
 + proc; simplify.
   transitivity {1}
    { (c,r) <@ W64x8.R.Ops.subcR(a,b,c); }
@@ -231,8 +231,8 @@ proc.
 while (cond = x /\ b = z /\ i <= dnlimbs 
   /\ (forall j, 0 <= j < i => a.[j] = if cond then z.[j] else y.[j])
   /\ (forall j, i <= j < dnlimbs => a.[j] = y.[j])) (dnlimbs - i). progress.
-wp.  skip.  progress. smt().   smt(@Array14). smt(@Array14). smt(). wp.  skip. progress. smt(@Array14). smt().
-apply Array14.ext_eq. progress. smt(@Array14). 
+wp.  skip.  progress. smt().   smt(@Array64). smt(@Array64). smt(). wp.  skip. progress. smt(@Array64). smt().
+apply Array64.ext_eq. progress. smt(@Array64). 
 qed.
 
 
@@ -240,17 +240,17 @@ qed.
 (*   phoare[ M.bn_set0 : true  ==> W64x4.valR res = 0 ] = 1%r. *)
 (* proc. *)
 (* while (i <= nlimbs  *)
-(*   /\ (forall j, 0 <= j < i => a.[j]%Array7 = W64.zero)) (nlimbs - i). progress. *)
-(* wp.  skip.  progress. smt().  smt(@Array7). smt(). wp.  skip. progress. smt(). smt(). *)
+(*   /\ (forall j, 0 <= j < i => a.[j]%Array32 = W64.zero)) (nlimbs - i). progress. *)
+(* wp.  skip.  progress. smt().  smt(@Array32). smt(). wp.  skip. progress. smt(). smt(). *)
 (* rewrite - zeroRE. congr. *)
-(* apply Array7.ext_eq. progress.  rewrite H1. smt().  *)
-(* rewrite /zeroR. smt(@Array7). *)
+(* apply Array32.ext_eq. progress.  rewrite H1. smt().  *)
+(* rewrite /zeroR. smt(@Array32). *)
 (* qed. *)
 
 
 require import List.
 
-op oneR : R = (of_list W64.zero (W64.one :: nseq (nlimbs - 1) W64.zero ))%Array7.
+op oneR : R = (of_list W64.zero (W64.one :: nseq (nlimbs - 1) W64.zero ))%Array32.
 
     (* TODO: nlimbs specific *)
 lemma oneRE: ImplZZ oneR 1.
@@ -259,14 +259,14 @@ do? (rewrite range_ltn; first by trivial ).
 simplify. rewrite range_geq. auto.
 do rewrite big_consT.
 rewrite big_nil.
- have -> : dig ((of_list W64.zero (W64.one :: nseq (nlimbs - 1) W64.zero)))%Array7 0 = 1.
+ have -> : dig ((of_list W64.zero (W64.one :: nseq (nlimbs - 1) W64.zero)))%Array32 0 = 1.
  simplify. smt(@Int).
- have q : forall x, 0 < x < nlimbs => dig ((of_list W64.zero (W64.one :: nseq (nlimbs - 1) W64.zero)))%Array7 x = 0.
+ have q : forall x, 0 < x < nlimbs => dig ((of_list W64.zero (W64.one :: nseq (nlimbs - 1) W64.zero)))%Array32 x = 0.
  move => x xp. rewrite /dig.
-   have ->: to_uint ((of_list W64.zero (W64.one :: nseq (nlimbs - 1) W64.zero)).[x])%Array7 = 0. 
+   have ->: to_uint ((of_list W64.zero (W64.one :: nseq (nlimbs - 1) W64.zero)).[x])%Array32 = 0. 
     do? (rewrite nseqS'; first by trivial). simplify. 
    rewrite nseq0. 
-  have -> : (of_list W64.zero [W64.one; W64.zero; W64.zero; W64.zero; W64.zero]).[x]%Array7 = W64.zero. 
+  have -> : (of_list W64.zero [W64.one; W64.zero; W64.zero; W64.zero; W64.zero]).[x]%Array32 = W64.zero. 
 rewrite get_of_list. smt().
 smt(@List).  smt(@W64). smt().
 do? (rewrite q; first smt()). auto.
@@ -277,13 +277,13 @@ lemma bn_set1_correct :
   phoare[ M.bn_set1 : true  ==> W64x4.valR res = 1 ] = 1%r.
 proc.
 while (0 < i <= nlimbs 
-  /\ (forall j, 1 <= j < i => a.[j]%Array7 = W64.zero) /\ a.[0]%Array7 = W64.one) (nlimbs - i). progress.
-wp.  skip.  progress. smt(). smt().  smt(@Array7). smt(@Array7). smt(). wp.  skip. progress. smt(@Array7). smt().
+  /\ (forall j, 1 <= j < i => a.[j]%Array32 = W64.zero) /\ a.[0]%Array32 = W64.one) (nlimbs - i). progress.
+wp.  skip.  progress. smt(). smt().  smt(@Array32). smt(@Array32). smt(). wp.  skip. progress. smt(@Array32). smt().
 rewrite - oneRE. congr.
-apply Array7.ext_eq. progress.  
+apply Array32.ext_eq. progress.  
 case (x = 0). progress. progress.
 rewrite H2. smt(). 
-rewrite /oneR. smt(@Array7 @List).
+rewrite /oneR. smt(@Array32 @List).
 qed.
 
 
@@ -294,8 +294,8 @@ proc.
 while (a = x /\ i <= dnlimbs 
   /\ (forall j, 0 <= j < i => r.[j] = x.[j])
   ) (dnlimbs - i). progress.
-wp.  skip.  progress. smt(). smt(@Array14). smt(). wp.  skip. progress. smt(). smt().
-apply Array14.ext_eq. progress. smt(). 
+wp.  skip.  progress. smt(). smt(@Array64). smt(). wp.  skip. progress. smt(). smt().
+apply Array64.ext_eq. progress. smt(). 
 qed.
 
 
@@ -303,10 +303,10 @@ lemma bn_copy_correct x :
   phoare[ M.bn_copy :  arg = x  ==> res = x ] = 1%r.
 proc.
 while (a = x /\ i <= nlimbs 
-  /\ (forall j, 0 <= j < i => r.[j]%Array7 = x.[j]%Array7)
+  /\ (forall j, 0 <= j < i => r.[j]%Array32 = x.[j]%Array32)
   ) (dnlimbs - i). progress.
-wp.  skip.  progress. smt(). smt(@Array7). smt(). wp.  skip. progress. smt(). smt().
-apply Array7.ext_eq. progress. smt(). 
+wp.  skip.  progress. smt(). smt(@Array32). smt(). wp.  skip. progress. smt(). smt().
+apply Array32.ext_eq. progress. smt(). 
 qed.
 
 
@@ -342,7 +342,7 @@ lemma bn_div2_correct z :
 proc. sp.
 while (aux = dnlimbs /\ i <= dnlimbs /\ forall j, 0 <= j < i => r.[j] = x.[dnlimbs + j]) (dnlimbs - i). 
 progress. wp. skip. progress.
-smt(). smt(@Array14). smt(). skip. progress.
+smt(). smt(@Array64). smt(). skip. progress.
 smt(). smt().
 have ->:  W64x8.modulusR  = W64x8.M^dnlimbs.  rewrite /R.bn_modulus. auto. 
 have ->: (R2.bnk (2*dnlimbs) x{hr})%R2 = valR2 x{hr}. auto.
@@ -365,9 +365,9 @@ lemma bn_shrink_correct a  :
   phoare[ M.bn_shrink : arg = a  ==> W64x4.valR res = W64x8.valR a %% W64x4.modulusR ] = 1%r.
 proc.
 sp.
-while (i <= nlimbs /\ forall j, 0 <= j < i => r.[j]%Array7 = x.[j]%Array14) (nlimbs - i). 
+while (i <= nlimbs /\ forall j, 0 <= j < i => r.[j]%Array32 = x.[j]%Array64) (nlimbs - i). 
 progress. wp. skip. progress.
-smt(). smt(@Array7). smt(). skip. progress.
+smt(). smt(@Array32). smt(). skip. progress.
 smt(). smt(). 
 rewrite /W64x4.modulusR. auto.
 rewrite W64x8.R.bn_mod. auto. 
@@ -386,34 +386,34 @@ lemma bn_expand_correct : forall a,
    move => a.
    proc.
    sp. 
-    seq 1 : (a = x /\ i = nlimbs /\ forall i, i < nlimbs => r.[i] = x.[i]%Array7).
-    while (i <= nlimbs /\ forall j, 0 <= j < i => r.[j] = x.[j]%Array7). wp.  skip. progress.
-    smt(). smt(@Array7 @Array14). skip. progress.
-    smt().  smt(). smt(@Array14 @Array7). 
-    seq 2 : (a = x /\  (forall j, 0 <= j < nlimbs => r.[j]%Array14 = x.[j]%Array7)
+    seq 1 : (a = x /\ i = nlimbs /\ forall i, i < nlimbs => r.[i] = x.[i]%Array32).
+    while (i <= nlimbs /\ forall j, 0 <= j < i => r.[j] = x.[j]%Array32). wp.  skip. progress.
+    smt(). smt(@Array32 @Array64). skip. progress.
+    smt().  smt(). smt(@Array64 @Array32). 
+    seq 2 : (a = x /\  (forall j, 0 <= j < nlimbs => r.[j]%Array64 = x.[j]%Array32)
          /\ (forall j, nlimbs <= j < 2*nlimbs => r.[j] = W64.zero)).     
     while (a = x /\ nlimbs <= i <= 2*nlimbs 
-         /\ (forall j, 0 <= j < nlimbs => r.[j]%Array14 = x.[j]%Array7)
+         /\ (forall j, 0 <= j < nlimbs => r.[j]%Array64 = x.[j]%Array32)
          /\ (forall j, nlimbs <= j < i => r.[j] = W64.zero) ). wp.  skip. progress.
     smt(). smt().
     have z : i{hr} <> j. smt(). 
-    rewrite - H1. auto.  smt(@Array7 @Array14).
-    case (j = i{hr}). smt(@Array7 @Array14).
+    rewrite - H1. auto.  smt(@Array32 @Array64).
+    case (j = i{hr}). smt(@Array32 @Array64).
     progress.
     have : j < i{hr}.  smt().
     progress.
     rewrite - (H2 j).  smt().
-    smt(@Array7 @Array14). wp. 
+    smt(@Array32 @Array64). wp. 
     skip.  progress.
-    smt(@Array7 @Array14). smt(). smt(). 
+    smt(@Array32 @Array64). smt(). smt(). 
     skip.  progress.
-    have -> : valR r{hr} = (bn_seq ((to_list r{hr}))%Array14).
+    have -> : valR r{hr} = (bn_seq ((to_list r{hr}))%Array64).
     apply W64x8.R.bn2seq. 
     rewrite /to_list.
     have -> : dnlimbs = nlimbs + nlimbs. smt().
     rewrite mkseq_add. auto. auto.
     have -> : mkseq (fun (i0 : int) => r{hr}.[i0]) nlimbs 
-      = mkseq (fun (i0 : int) => x{hr}.[i0]%Array7) nlimbs.
+      = mkseq (fun (i0 : int) => x{hr}.[i0]%Array32) nlimbs.
     apply eq_in_mkseq. progress. 
     simplify.
     have ->: mkseq (fun (i0 : int) => r{hr}.[nlimbs + i0]) nlimbs
@@ -471,7 +471,7 @@ have -> : W64x8.modulusR = 2 ^ (2 * k{2}). smt(@Ring). smt().
 seq 1 1 : (valR a{1} = a{2} /\ valR r{1} = r{2} /\ ImplZZ p{1} P /\ k{2} = 64 * nlimbs
     /\ W64x8.valR2 xr{1} = xr{2} /\  valR xrfd{1} =  xrf{2}   ).
 ecall {1} (bn_shrink_correct xrf{1}). wp. skip. progress. rewrite H0.  
-have ->: W64x4.modulusR = Fp_w64x4_spec.M. rewrite /W64x4.modulusR. smt(@Ring). auto.
+have ->: W64x4.modulusR = Fp_w64x4_spec.M. rewrite /W64x4.modulusR. rewrite /M. smt(@Ring). rewrite /M. smt(@Ring). 
 seq 1 1 : (valR a{1} = a{2} /\ valR r{1} = r{2} /\ ImplZZ p{1} P /\ k{2} = 64 * nlimbs
     /\ W64x8.valR2 xr{1} = xr{2} /\ valR xrfd{1} = xrf{2} 
     /\  W64x8.valR xrfn{1} = xrfn{2}).
@@ -510,7 +510,7 @@ equiv bnreduce_spec:
  M.bn_breduce ~ ASpecFp.redm:
   valR a{1} = a{2}
   /\ ImplZZ p{1} P
-  /\ valR r{1} = (4 ^ (64 * nlimbs) %/ P) 
+  /\ valR r{1} = (ri P (64 * nlimbs))  
   /\ 0 < P < W64x4.modulusR
   /\ 0 <= a{2} < P * P
   /\ 0 < P < 2 ^ (64 * nlimbs)
@@ -525,7 +525,7 @@ symmetry. transitivity ASpecFp.redm
  (={arg} ==> res{1} = res{2} %% W64x4.modulusR)
  (valR a{2} = a{1}
   /\ ImplZZ p{2} P
-  /\ valR r{2} = (4 ^ (64 * nlimbs) %/ P) 
+  /\ valR r{2} =  (ri P (64 * nlimbs))  
   /\ 0 < P < W64x4.modulusR
   /\ 0 <= a{1} < P * P
   /\ 0 < P < 2 ^ (64 * nlimbs)
@@ -539,20 +539,17 @@ transitivity CSpecFp.redm
  /\  W64x4.valR p{1} = P
  /\  k{2} = 64 * nlimbs
    ==>  (W64x4.valR res{1}) = res{2}  %% W64x4.modulusR)
- (={a} /\ r{1} = (4 ^ k{1} %/ P) 
+ (={a} /\ r{1} = (ri P k{1}) 
   /\ 0 < P < W64x4.modulusR
   /\ 0 <= a{1} < P * P
   /\ 0 < P < 2 ^ k{1} 
   /\ 0 <= k{1} ==> ={res}). 
 move => &1 &2 q. 
 exists (valR a{1} , valR r{1} , 64 * nlimbs). split. smt(). 
-split. smt(). split.  
-have ->: (valR a{1}, valR r{1}, 64 * nlimbs).`2 = valR r{1}. auto.
-have ->: (valR a{1}, valR r{1}, 64 * nlimbs).`3 = 64 * nlimbs. auto.
-rewrite q. smt().  
- split.  smt(). 
+split. smt(). split. smt().   split.  smt(). 
 split. smt(). split. split. smt().  move => ?. 
- have ->: Fp_w64x4_spec.M = W64x4.modulusR. clear q. rewrite /W64x4.modulusR. smt(@Ring). 
+have ->: (valR a{1}, valR r{1}, 64 * nlimbs).`3 = 64 * nlimbs. smt().
+ have ->: 2 ^ (dnlimbs * nlimbs) = W64x4.modulusR. clear q. rewrite /W64x4.modulusR. smt(@Ring).
 smt(). smt(). auto.
 conseq breduce_cspec.
 symmetry. conseq redm_eq. auto. auto.
@@ -569,7 +566,7 @@ equiv mulm_cspec:
   /\ valR a{1} < P
   /\ valR b{1} < P
   /\ ImplZZ p{1} P
-  /\ valR r{1} = (4 ^ (64 * nlimbs) %/ P) 
+  /\ valR r{1} = ri P (64 * nlimbs)
    ==> valR res{1} =  res{2} .
 proc. 
 call bnreduce_spec.
@@ -579,11 +576,11 @@ move => &1 &2 H1. split. smt().
 move => q1 r1 r2 r3 . split. simplify. rewrite - r3.
 smt(@W64x4 @W64x8).
    split.  simplify. smt().
-split. rewrite H1. trivial.
+split. smt().
 split.  smt (P_pos bnk_cmp).
 split.  smt (P_pos bnk_cmp).
 split.  split. smt (P_pos).
-have -> : Fp_w64x4_spec.M = W64x4.modulusR. rewrite /W64x4.modulusR. smt(@Ring).
+have -> :  2 ^ (dnlimbs * nlimbs) = W64x4.modulusR. rewrite /W64x4.modulusR. smt(@Ring).
 smt(ppos). smt(W64x8.R.bnk_cmp).
 qed.
 
@@ -648,20 +645,24 @@ rewrite /W64x4.modulusR.
 split. apply bs2int_ge0. 
 have ->: `|W64x8.M ^ nlimbs| = W64x8.M ^ nlimbs. smt(@Int).
 have xx : bs2int x < 2 ^ (64*nlimbs).  
-  have o : forall n (s : bool list),  n = size s => bs2int s < 2 ^ n. smt(bs2int_le2Xs).
-  apply o. smt().
+    have o : forall n (s : bool list),  n = size s => bs2int s < 2 ^ n. smt(bs2int_le2Xs).
+(* have -> : Fp_w64x4_spec.M = W64x4.modulusR. rewrite /W64x4.modulusR. smt(@Ring). *)
+(* rewrite /W64x4.modulusR. *)
+
+    (* ??? *)
+have ->:  (dnlimbs * nlimbs) = 2048. smt().
+clear o. rewrite -H. smt(bs2int_le2Xs).
 
 have <- : 2 ^ (64*nlimbs) = W64x8.M ^ nlimbs. smt(@Ring).
-auto. 
+move => ?. assumption.
 smt(bs2intK). qed.
 realize bitsr_rbits. 
 rewrite /Rbits. rewrite /bitsR.
 progress.
 rewrite int2bsK. auto. simplify. progress. smt(bnk_cmp).
 have : 0 <= valR  x < W64x4.M ^ nlimbs.
-rewrite /valR. 
 apply (bnk_cmp nlimbs).
-progress. smt(@Ring).
+smt(@Ring).
 smt(@W64x4).
 qed.
 realize exp_prop7. progress.
@@ -698,8 +699,8 @@ rewrite bnk_ofintK. auto. smt(@Ring P_pos). qed.
 module MultM = {
   proc ith_bit = M.ith_bit
   proc swapr   = M.swapr
-  proc opr (p:W64.t Array7.t, a:W64.t Array7.t,
-             b:W64.t Array7.t) : W64.t Array7.t = {
+  proc opr (p:W64.t Array32.t, a:W64.t Array32.t,
+             b:W64.t Array32.t) : W64.t Array32.t = {
     var r;
     r <@ M.mulm(R,p,a,b);
     return r;
@@ -719,69 +720,69 @@ seq 2 0 : (i{1} = 0 /\ a{2} = x{1} /\ b{2} = y{1} /\ swap_0{1} = as_w64 c{2} /\
 wp. skip. progress. smt(@W64). smt(@W64).
 while {1} (0 <= i{1} /\ ((as_bool swap_0{1} => mask{1} = (of_int 18446744073709551615)%W64 )
               /\ (as_bool swap_0{1} = false => mask{1} = (of_int 0)%W64)) 
-   /\ (forall j, 0 <= j < i{1} => (x{1}.[j])%Array7 = (if as_bool swap_0{1} then (b{2}.[j]) else (a{2}.[j]))%Array7 )  
-   /\ (forall j, 0 <= j < i{1} => (y{1}.[j])%Array7 = (if as_bool swap_0{1} then (a{2}.[j]) else (b{2}.[j]))%Array7 )  
-   /\ (forall j, i{1} <= j => (x{1}.[j])%Array7 =  (a{2}.[j]))%Array7
-   /\ (forall j, i{1} <= j => (y{1}.[j])%Array7 =  (b{2}.[j]))%Array7
+   /\ (forall j, 0 <= j < i{1} => (x{1}.[j])%Array32 = (if as_bool swap_0{1} then (b{2}.[j]) else (a{2}.[j]))%Array32 )  
+   /\ (forall j, 0 <= j < i{1} => (y{1}.[j])%Array32 = (if as_bool swap_0{1} then (a{2}.[j]) else (b{2}.[j]))%Array32 )  
+   /\ (forall j, i{1} <= j => (x{1}.[j])%Array32 =  (a{2}.[j]))%Array32
+   /\ (forall j, i{1} <= j => (y{1}.[j])%Array32 =  (b{2}.[j]))%Array32
  ) (nlimbs - i{1} + 1).
 progress. wp.  skip.  progress.   smt().
-case (j <  i{hr}). progress. smt(@Array7).
+case (j <  i{hr}). progress. smt(@Array32).
 progress.
 have : j = i{hr}. smt().
 progress.
 have ->: (x{hr}.[i{hr} <-
-    x{hr}.[i{hr}] `^` (x{hr}.[i{hr}] `^` y{hr}.[i{hr}] `&` mask{hr})].[i{hr}])%Array7
- = (x{hr}.[i{hr}] `^` (x{hr}.[i{hr}] `^` y{hr}.[i{hr}] `&` mask{hr}))%Array7. smt(@Array7).
+    x{hr}.[i{hr}] `^` (x{hr}.[i{hr}] `^` y{hr}.[i{hr}] `&` mask{hr})].[i{hr}])%Array32
+ = (x{hr}.[i{hr}] `^` (x{hr}.[i{hr}] `^` y{hr}.[i{hr}] `&` mask{hr}))%Array32. smt(@Array32).
 case (as_bool swap_0{hr}). progress.
 rewrite H4. auto.  rewrite H0. auto. rewrite H5. auto. rewrite - ones64. 
-have -> : ((a{m}.[i{hr}])%Array7 `^` (b{m}.[i{hr}])%Array7 `&`
- (of_int W64.max_uint)%W64) = a{m}.[i{hr}]%Array7 `^` ((b{m}.[i{hr}])%Array7 `&`
+have -> : ((a{m}.[i{hr}])%Array32 `^` (b{m}.[i{hr}])%Array32 `&`
+ (of_int W64.max_uint)%W64) = a{m}.[i{hr}]%Array32 `^` ((b{m}.[i{hr}])%Array32 `&`
  (of_int W64.max_uint)%W64).
-pose x := a{m}.[i{hr}]%Array7.
-pose y := b{m}.[i{hr}]%Array7.
+pose x := a{m}.[i{hr}]%Array32.
+pose y := b{m}.[i{hr}]%Array32.
 pose z := (of_int W64.max_uint)%W64.
 rewrite andwDl.
 have ->: (x `&` z) = x. smt (W64.andw1_s).
 auto.
-have ->: ((b{m}.[i{hr}])%Array7 `&` (of_int W64.max_uint)%W64) = ((b{m}.[i{hr}])%Array7). 
-pose y := b{m}.[i{hr}]%Array7.
+have ->: ((b{m}.[i{hr}])%Array32 `&` (of_int W64.max_uint)%W64) = ((b{m}.[i{hr}])%Array32). 
+pose y := b{m}.[i{hr}]%Array32.
 pose z := (of_int W64.max_uint)%W64.
 smt (W64.andw1_s).
 smt(@W64).
 progress. rewrite H4. auto.  rewrite H1. smt(). auto. 
-case (j <  i{hr}). progress. smt(@Array7).
+case (j <  i{hr}). progress. smt(@Array32).
 progress.
 have : j = i{hr}. smt().
 progress.
 have ->: (y{hr}.[i{hr} <-
-   y{hr}.[i{hr}] `^` (x{hr}.[i{hr}] `^` y{hr}.[i{hr}] `&` mask{hr})].[i{hr}])%Array7
- = (y{hr}.[i{hr}] `^` (x{hr}.[i{hr}] `^` y{hr}.[i{hr}] `&` mask{hr}))%Array7. smt(@Array7).
+   y{hr}.[i{hr}] `^` (x{hr}.[i{hr}] `^` y{hr}.[i{hr}] `&` mask{hr})].[i{hr}])%Array32
+ = (y{hr}.[i{hr}] `^` (x{hr}.[i{hr}] `^` y{hr}.[i{hr}] `&` mask{hr}))%Array32. smt(@Array32).
 case (as_bool swap_0{hr}). progress.
 rewrite H4. auto.  rewrite H0. auto. rewrite H5. auto. rewrite - ones64. 
-have -> : ((a{m}.[i{hr}])%Array7 `^` (b{m}.[i{hr}])%Array7 `&`
- (of_int W64.max_uint)%W64) = a{m}.[i{hr}]%Array7 `^` ((b{m}.[i{hr}])%Array7 `&`
+have -> : ((a{m}.[i{hr}])%Array32 `^` (b{m}.[i{hr}])%Array32 `&`
+ (of_int W64.max_uint)%W64) = a{m}.[i{hr}]%Array32 `^` ((b{m}.[i{hr}])%Array32 `&`
  (of_int W64.max_uint)%W64). 
-pose x := a{m}.[i{hr}]%Array7.
-pose y := b{m}.[i{hr}]%Array7.
+pose x := a{m}.[i{hr}]%Array32.
+pose y := b{m}.[i{hr}]%Array32.
 pose z := (of_int W64.max_uint)%W64.
 rewrite andwDl.
 have ->: (x `&` z) = x. smt (W64.andw1_s).
 auto.
-have ->: ((b{m}.[i{hr}])%Array7 `&` (of_int W64.max_uint)%W64) = ((b{m}.[i{hr}])%Array7).
-pose y := b{m}.[i{hr}]%Array7.
+have ->: ((b{m}.[i{hr}])%Array32 `&` (of_int W64.max_uint)%W64) = ((b{m}.[i{hr}])%Array32).
+pose y := b{m}.[i{hr}]%Array32.
 pose z := (of_int W64.max_uint)%W64.
 smt (W64.andw1_s).
 smt(@W64).
 progress. rewrite H4. auto.  rewrite H1. smt(). smt(@W64).
-smt(@Array7). smt(@Array7). smt().
+smt(@Array32). smt(@Array32). smt().
 skip. progress. smt().   smt().   smt(). 
 case (c{2} = false). progress.  
-apply Array7.ext_eq.  progress. rewrite H5. progress. smt(). rewrite /as_bool. rewrite /as_w64. simplify. smt(@W64).
-apply Array7.ext_eq.  progress. rewrite H6. progress. smt(). rewrite /as_bool. rewrite /as_w64. simplify. smt(@W64).
+apply Array32.ext_eq.  progress. rewrite H5. progress. smt(). rewrite /as_bool. rewrite /as_w64. simplify. smt(@W64).
+apply Array32.ext_eq.  progress. rewrite H6. progress. smt(). rewrite /as_bool. rewrite /as_w64. simplify. smt(@W64).
 progress. have ->: c{2} = true. smt(). simplify.
 progress. 
-apply Array7.ext_eq.  progress. rewrite H5. progress. smt(). rewrite /as_bool. rewrite /as_w64. simplify. smt(@W64).
-apply Array7.ext_eq.  progress. rewrite H6. progress. smt(). rewrite /as_bool. rewrite /as_w64. simplify. smt(@W64).
+apply Array32.ext_eq.  progress. rewrite H5. progress. smt(). rewrite /as_bool. rewrite /as_w64. simplify. smt(@W64).
+apply Array32.ext_eq.  progress. rewrite H6. progress. smt(). rewrite /as_bool. rewrite /as_w64. simplify. smt(@W64).
 qed.
 
 
@@ -830,14 +831,14 @@ progress. smt(@Zp @W64x4).
 qed.
 
 module MM = {
-  proc ith_bit (kk:W64.t Array7.t, ctr:W64.t) : W64.t = {
+  proc ith_bit (kk:W64.t Array32.t, ctr:W64.t) : W64.t = {
     var bit:W64.t;
     var c1:W64.t;
     var c2:W64.t;
     var r:W64.t;
     c1 <- (ctr `>>` (W8.of_int 6));
     c2 <- (ctr - (c1 * (W64.of_int 64)));
-    r <- kk.[(W64.to_uint c1)]%Array7;
+    r <- kk.[(W64.to_uint c1)]%Array32;
     bit <@ IB.ith_bit64 (r, c2);
     return (bit);
   }
@@ -900,7 +901,7 @@ progress. smt(). smt().
 symmetry. conseq ith_bit_lemmaEq. auto. auto.
 proc.
 seq 3 0 : (to_uint c1{1} = (to_uint ctr{1} %/ 64) /\ to_uint c2{1} = (to_uint ctr{1} %% 64) /\ to_uint ctr{1} = ctr{2}
-  /\ r{1} = kk{1}.[(to_uint ctr{1} %/ 64)]%Array7 /\ r{2} = kk{1} /\ 0 <= ctr{2} && ctr{2} < 64*nlimbs ).
+  /\ r{1} = kk{1}.[(to_uint ctr{1} %/ 64)]%Array32 /\ r{2} = kk{1} /\ 0 <= ctr{2} && ctr{2} < 64*nlimbs ).
 wp.  skip. progress.
 rewrite shr_div_le. auto. smt(@Ring).
 rewrite modzE.
@@ -933,25 +934,25 @@ rewrite /ith_bitR. rewrite /Rbits. rewrite /valR.
 rewrite /ith_bit.
 rewrite /as_word.
 rewrite /as_w64.
-have ->: (kk{1}.[to_uint ctr{1} %/ 64])%Array7.[to_uint ctr{1} %% 64]
+have ->: (kk{1}.[to_uint ctr{1} %/ 64])%Array32.[to_uint ctr{1} %% 64]
   = nth false (int2bs (64 * nlimbs) ((valR kk{1}))%W64x4) (to_uint ctr{1}) .
 rewrite - get_w2bits.
 rewrite - get_to_list.
-have -> : (W64.w2bits (nth witness ((to_list kk{1}))%Array7 (to_uint ctr{1} %/ 64)))
- = ((nth witness (map W64.w2bits (to_list kk{1}))%Array7 (to_uint ctr{1} %/ 64))).
+have -> : (W64.w2bits (nth witness ((to_list kk{1}))%Array32 (to_uint ctr{1} %/ 64)))
+ = ((nth witness (map W64.w2bits (to_list kk{1}))%Array32 (to_uint ctr{1} %/ 64))).
 rewrite - (nth_map witness witness W64.w2bits). progress.   smt(). smt(@W64x4).
 auto.
-have -> : (nth witness (map W64.w2bits ((to_list kk{1}))%Array7)
+have -> : (nth witness (map W64.w2bits ((to_list kk{1}))%Array32)
      (to_uint ctr{1} %/ 64))
- = (nth [] (map W64.w2bits ((to_list kk{1}))%Array7)
+ = (nth [] (map W64.w2bits ((to_list kk{1}))%Array32)
      (to_uint ctr{1} %/ 64)).
 rewrite (nth_change_dfl [] witness). progress.  smt(). smt(@W64x4 @List). auto.
-rewrite - (BitChunking.nth_flatten false 64 (map W64.w2bits ((to_list kk{1}))%Array7) (to_uint ctr{1})).
+rewrite - (BitChunking.nth_flatten false 64 (map W64.w2bits ((to_list kk{1}))%Array32) (to_uint ctr{1})).
 rewrite  List.allP. progress.
-have : exists z, z \in ((to_list kk{1}))%Array7 /\ x = W64.w2bits z.
+have : exists z, z \in ((to_list kk{1}))%Array32 /\ x = W64.w2bits z.
 apply mapP. auto. elim. progress.
-have ->: (flatten (map W64.w2bits ((to_list kk{1}))%Array7))  = (int2bs (64*nlimbs) ((valR kk{1}))%W64x4).
-have -> : (valR kk{1})%W64x4 = bs2int (flatten (map W64.w2bits ((to_list kk{1}))%Array7)).
+have ->: (flatten (map W64.w2bits ((to_list kk{1}))%Array32))  = (int2bs (64*nlimbs) ((valR kk{1}))%W64x4).
+have -> : (valR kk{1})%W64x4 = bs2int (flatten (map W64.w2bits ((to_list kk{1}))%Array32)).
 rewrite /bnk.
 do? (rewrite range_ltn; first by trivial).
 simplify. rewrite range_geq. auto. auto.
@@ -965,8 +966,10 @@ rewrite flatten_nil.
 rewrite cats0.
 do? rewrite bs2int_cat.
 simplify.
+have ->:  18446744073709551616 ^ 0 = 1. smt(@Ring).
+simplify.
 smt(@Ring).
-have ->: 64*nlimbs = size (flatten (map W64.w2bits ((to_list kk{1}))%Array7)).
+have ->: 64*nlimbs = size (flatten (map W64.w2bits ((to_list kk{1}))%Array32)).
 rewrite /to_list.
 do? (rewrite mkseqS'; first by trivial).
 rewrite mkseq0. simplify.
