w64x4/proof/Array32.ec
@@ -1,3 +1,6 @@
 require import JArray.
 
 clone export PolyArray as Array32  with op size <- 32.
+
+require import JModel.
+abbrev sbb_64 = subc_64.
